---
title: Random notes
description: 
published: true
date: 2021-08-30T04:13:46.971Z
tags: 
editor: markdown
---

# Random notes

I was reading the following two resources about summation identities:
1) Concrete Mathematics: A Foundation for Computer Science (2nd Ed) by Knuth and Patashnik section 2.3 Manipulation of Sums
2) this other resource [here][1] on summation algebra I randomly came across googling. 


CM is calling the **Distributive Law** as follows:

$\sum_{k \in K} c a_{k}=c \sum_{k \in K} a_{k}$

but the book on the algebra of summations calls it  **"The Second Constant Rule"**

$\sum_{i=1}^{N} a x_{i}=a \sum_{i=1}^{N} x_{i}$


CM is calling the **Associative Law** as follows:

$\sum_{k \in K}\left(a_{k}+b_{k}\right)=\sum_{k \in K} a_{k}+\sum_{k \in K} b_{k}$

but the other resource calls it **"The Distributive Rule of Summation Algebra"**

$\sum_{i=1}^{N}\left(x_{i}+y_{i}\right)=\sum_{i=1}^{N} x_{i}+\sum_{i=1}^{N} y_{i}$

I can see how **"The Second Constant Rule"** is 



  [1]: http://www.statpower.net/Content/310/Summation%20Algebra.pdf